



PES University, Bangalore

(Established Under Karnataka Act 16 of 2013)

Department of Science and Humanities

Engineering Mathematics - I (UE25MA141A)

Question Bank

Unit - 3: Partial Differential Equations

1. Eliminate the arbitrary function f from the equation:

$$z = f\left(\frac{xy}{z}\right)$$

and form the corresponding partial differential equation (PDE).

Answer: $px = qy$, where $p = \frac{\partial z}{\partial x}$ and $q = \frac{\partial z}{\partial y}$.

2. Form the partial differential equation by eliminating the arbitrary functions f and g in:

$$z = x^2 f(y) + y^2 g(x)$$

Answer: $xyz + 4z = 2px + 2qy$

3. Form the partial differential equation by eliminating the arbitrary functions f and g in:

$$z = f(x^3 + 2y) + g(x^3 - 2y)$$

Answer: $9x^5 t - 4xr + 8p = 0$

4. Solve the partial differential equation:

$$\frac{y^2 z}{x} \frac{\partial z}{\partial x} + xz \frac{\partial z}{\partial y} = y^2$$

Answer: $\Phi(x^2 - z^2, y^3 - x^3) = 0$

5. Solve the partial differential equation:

$$(x^2 + y^2 + yz) \frac{\partial z}{\partial x} + (x^2 + y^2 - zx) \frac{\partial z}{\partial y} = z(x + y)$$

Answer: $\Phi\left(2xz - \frac{z^2}{2}, x^2 + y^2 + z^2\right) = 0$

6. Solve the partial differential equation:

$$x(y^2 + z) \frac{\partial z}{\partial x} + y(x^2 + z) \frac{\partial z}{\partial y} = z(x^2 - y^2)$$

Answer: $\Phi\left(x^2 - y^2 - 2z, \frac{xz}{y}\right) = 0$

Solve the following by the method of the separation of variables
(Problems 7,8, and 9)

7. $3\frac{\partial u}{\partial x} + 2\frac{\partial u}{\partial y} = 0$, given $u(x, 0) = e^{-x}$

Answer: $u = e^{-\frac{1}{2}(2x-3y)}$

8. $4\frac{\partial u}{\partial x} + \frac{\partial u}{\partial y} = 3u$, given $u = 3e^{-y} - e^{-5y}$ when $x = 0$.

Hine: Write u as the sum of two solutions. That is, $u = C_1 e^{\frac{\lambda_1}{4}x + (3-\lambda_1)y} + C_2 e^{\frac{\lambda_2}{4}x + (3-\lambda_2)y}$

Answer: $u = 3e^{x-y} - e^{2x-3y}$

9. $\frac{\partial^2 u}{\partial x^2} - 2\frac{\partial u}{\partial x} + \frac{\partial u}{\partial y} = 0$.

Answer: $u = \left(C_1 e^{(1+\sqrt{1+\lambda})x} + C_2 e^{(1-\sqrt{1+\lambda})x} \right) e^{-\lambda y}$

10. Solve $(D^3 + D^2 D' - D D'^2 - D'^3)z = 0$.

Answer: $z = \phi_1(x+y) + x\phi_2(x-y) + \phi_3(x-y)$

11. Solve $[D^3 - D^2 D' - 4D(D')^2 + (4D')^3]z = 0$.

Answer: $z = \phi_1(x+y) + \phi_2(2x-y) + \phi_3(2x+y)$.

12. Solve $[2D^2 + 5DD' + 3(D')^2 + D + D']z = 0$.

Answer: $z = \phi_1(x-y) + e^{-x/2}\phi_2(3x-2y)$.

13. Solve the partial differential equation: $[D^2 + 3DD' + 2(D')^2]z = e^{x-y}$.

Answer:

C.F.: $z = \phi_1(x-y) + \phi_2(2x-y)$, P.I.: $-xe^{x-y}$ or $-ye^{x-y}$.

14. Solve the partial differential equation: $[3D^2 + 7DD' + 2(D')^2]z = 3x^2 + 2y^2$.

Answer:

$$z = \phi_1(2x-y) + \phi_2(x-3y) + \frac{x^2}{324}[113x^2 + 108y^2 - 168xy].$$

15. Solve the partial differential equation: $[4D^2 + 4DD' + (D')^2]z = 4y \cos(2x)$.

Answer:

$$z = \phi_1(x-2y) + x\phi_2(x-2y) + \frac{1}{8}[\sin(2x) - 2y \cos(2x)].$$